txn-data-consistency/Reductions.thy
@@ -26,8 +26,8 @@ text \<open>Condition for commuting a pair of events\<close>
 definition left_commute :: "('e, 's) ES \<Rightarrow> 'e \<Rightarrow> 'e \<Rightarrow> bool" where
   "left_commute E e1 e2 \<longleftrightarrow> strans E e2 O strans E e1 \<subseteq> strans E e1 O strans E e2"
 
-abbreviation right_commute where
-  "right_commute E e1 e2 \<equiv> left_commute e2 e1"
+abbreviation right_commute :: "('e, 's) ES \<Rightarrow> 'e \<Rightarrow> 'e \<Rightarrow> bool" where
+  "right_commute E e1 e2 \<equiv> left_commute E e2 e1"
 
 
 abbreviation cwit :: "('e, 's) ES \<Rightarrow> 's \<Rightarrow> 'e \<Rightarrow> 'e \<Rightarrow> 's \<Rightarrow> 's" where
@@ -166,6 +166,61 @@ lemma reach_reduced_invariants:
 
 
 text \<open>More useful rules TBA.\<close>
+
+thm "wf_induct_rule"
+
+lemma bad_exec_reducable_to_Good:
+  assumes
+    \<open>wf mes\<close>
+    \<open>valid_exec E ef\<close>
+    \<open>ef \<notin> Good\<close>
+    \<open>\<And>ef. \<lbrakk> valid_exec E ef; ef \<notin> Good \<rbrakk> \<Longrightarrow> (\<exists>ef'. E: ef \<rhd> ef' \<and> (ef' \<in> Good \<or> (ef', ef) \<in> mes))\<close>
+  shows
+    \<open>\<exists>ef' \<in> Good. E: ef \<rhd>\<^sup>+ ef'\<close>
+  using assms(1-3)
+proof (induction ef rule: wf_induct_rule)
+  case (less x)
+  then show ?case using assms(4) sorry
+qed
+
+
+\<comment> \<open>measure 1\<close>
+
+definition inverted_pairs :: "('s \<Rightarrow> 'a :: linorder) \<Rightarrow> ('e, 's) exec_frag \<Rightarrow> (nat \<times> nat) set" where
+  "inverted_pairs P ef =
+    {(i, j) | i j sl. i < j \<and> j < length sl \<and> P (sl ! i) > P (sl ! j) \<and> sl = states_of_efrag ef}"
+
+\<comment> \<open>measure 2\<close>
+definition closest_pair_distance :: "(nat \<times> nat) set \<Rightarrow> nat" where
+  "closest_pair_distance id_pairs \<equiv> Min {j - i | j i. (i, j) \<in> id_pairs}"
+
+abbreviation measure_func :: "('b \<Rightarrow> nat) \<Rightarrow> (('a, 'b) exec_frag \<times> ('a, 'b) exec_frag) set" where
+  "measure_func P \<equiv> measures [card o (inverted_pairs P), closest_pair_distance o (inverted_pairs P)]"
+
+definition Good_wrt where
+  "Good_wrt P \<equiv> {ef | ef. let sl = states_of_efrag ef in
+      \<forall>i j. i < j \<and> j < length sl \<longrightarrow> P (sl ! i) \<le> P (sl ! j)}"
+
+lemma reducable_exec:
+  fixes P :: "'s \<Rightarrow> nat"
+  assumes
+    \<open>valid_exec E ef\<close>
+    \<open>ef \<notin> Good_wrt P\<close>
+  shows
+    \<open>\<exists>ef'. E: ef \<rhd> ef' \<and> (ef', ef) \<in> measure_func P\<close>
+  sorry
+  
+
+lemma reducable_to_Good_exec:
+  fixes P :: "'s \<Rightarrow> nat"
+  assumes
+    \<open>valid_exec E ef\<close>
+    \<open>ef \<notin> Good_wrt P\<close>
+  shows
+    \<open>\<exists>ef' \<in> Good_wrt P. E: ef \<rhd>\<^sup>+ ef'\<close>
+  using assms
+  apply (auto dest!: reducable_exec[where P=P])
+  sorry
 
 
 end
