txn-data-consistency/Partial_Order_Reduction.thy
@@ -1,0 +1,199 @@
+section \<open>Partial order reduction\<close>
+
+theory Partial_Order_Reduction
+  imports "EP+_TCCv" Reductions
+begin
+
+\<comment> \<open>read_invoke (all except write_done independent)\<close>
+lemma read_invoke_read_invoke_indep:
+  "cl \<noteq> cl' \<Longrightarrow> left_commute tps (RInvoke cl keys) (RInvoke cl' keys')"
+  apply (auto simp add: left_commute_def tps_trans_defs del: equalityI)
+  apply (rule relcompI, auto)
+  by (simp add: fun_upd_twist)
+
+lemma read_invoke_read_indep:
+  "cl \<noteq> cl' \<Longrightarrow> left_commute tps (RInvoke cl keys) (Read cl' k' v' t')"
+  apply (auto simp add: left_commute_def tps_trans_defs del: equalityI)
+  apply (rule relcompI, auto)
+  by (simp add: fun_upd_twist)
+
+lemma read_invoke_read_done_indep:
+  "cl \<noteq> cl' \<Longrightarrow> left_commute tps (RInvoke cl keys) (RDone cl' kv_map' sn' u''')"
+  apply (auto simp add: left_commute_def tps_trans_defs get_ctx_defs del: equalityI)
+  apply (rule relcompI, auto)
+  by (simp add: fun_upd_twist)
+
+lemma read_invoke_write_invoke_indep:
+  "cl \<noteq> cl' \<Longrightarrow> left_commute tps (RInvoke cl keys) (WInvoke cl' kv_map')"
+  apply (auto simp add: left_commute_def tps_trans_defs del: equalityI)
+  apply (rule relcompI, auto)
+  by (simp add: fun_upd_twist)
+
+lemma read_invoke_write_commit_indep:
+  "cl \<noteq> cl' \<Longrightarrow> left_commute tps (RInvoke cl keys) (WCommit cl' kv_map' cts' sn' u''')"
+  apply (auto simp add: left_commute_def tps_trans_defs del: equalityI)
+  apply (rule relcompI, auto)
+  apply (simp add: fun_upd_twist)
+  by (metis domI option.inject)
+
+lemma read_invoke_register_read_indep:
+  "cl \<noteq> get_cl t' \<Longrightarrow> left_commute tps (RInvoke cl keys) (RegR k' t' i' rts')"
+  by (auto simp add: left_commute_def tps_trans_defs)
+
+lemma read_invoke_prepare_write_indep:
+  "cl \<noteq> get_cl_w t' \<Longrightarrow> left_commute tps (RInvoke cl keys) (PrepW k' t' v')"
+  by (auto simp add: left_commute_def tps_trans_defs)
+
+lemma read_invoke_commit_write_indep:
+  "cl \<noteq> get_cl_w t' \<Longrightarrow> left_commute tps (RInvoke cl keys) (CommitW k' t' v' cts')"
+  apply (auto simp add: left_commute_def tps_trans_defs del: equalityI; (rule relcompI)?, auto) sorry
+
+
+\<comment> \<open>read (all client events independent)\<close>
+lemma read_read_indep:
+  "cl \<noteq> cl' \<Longrightarrow> left_commute tps (Read cl k v t) (Read cl' k' v' t')"
+  apply (auto simp add: left_commute_def tps_trans_defs del: equalityI)
+  apply (rule relcompI, auto)
+  by (simp add: fun_upd_twist)
+
+lemma read_read_done_indep:
+  "cl \<noteq> cl' \<Longrightarrow> left_commute tps (Read cl k v t) (RDone cl' kv_map' sn' u''')"
+  apply (auto simp add: left_commute_def tps_trans_defs get_ctx_defs del: equalityI)
+  apply (rule relcompI, auto)
+  by (simp add: fun_upd_twist)
+
+lemma read_write_invoke_indep:
+  "cl \<noteq> cl' \<Longrightarrow> left_commute tps (Read cl k v t) (WInvoke cl' kv_map')"
+  apply (auto simp add: left_commute_def tps_trans_defs del: equalityI)
+  apply (rule relcompI, auto)
+  by (simp add: fun_upd_twist)
+
+lemma read_write_commit_indep:
+  "cl \<noteq> cl' \<Longrightarrow> left_commute tps (Read cl k v t) (WCommit cl' kv_map' cts' sn' u''')"
+  apply (auto simp add: left_commute_def tps_trans_defs del: equalityI)
+  apply (rule relcompI, auto)
+  apply (simp add: fun_upd_twist)
+  by (metis domI option.inject)
+
+lemma read_write_done_indep:
+  assumes "cl \<noteq> cl'"
+  shows "left_commute tps (Read cl k v t) (WDone cl' kv_map')"
+  using assms
+  apply (auto simp add: left_commute_def tps_trans_defs)
+  apply (rule relcompI, auto)
+  subgoal for s _ _ keys _ kv_map
+    proof -
+      have "let s' = s\<lparr>cls := (cls s)
+              (cl := cls s cl
+                 \<lparr>cl_state := RtxnInProg keys (kv_map(k \<mapsto> v)),
+                    cl_clock := Suc (max (cl_clock (cls s cl)) (svr_clock (svrs s k))),
+                    lst_map := (lst_map (cls s cl))(k := lst (svrs s k))\<rparr>)\<rparr>
+            in (\<lambda>ka. if kv_map' ka = None then lst_map (cls s' cl') ka
+                                else lst (svrs s' ka)) = 
+            (\<lambda>k. if kv_map' k = None then lst_map (cls s cl') k else lst (svrs s k))"
+        using assms by (auto simp add: Let_def)
+      then show ?thesis using assms by (auto simp add: Let_def fun_upd_twist)
+    qed
+    done
+
+lemma read_register_read_indep:
+  "cl \<noteq> get_cl t' \<Longrightarrow> left_commute tps (Read cl k v t_wr) (RegR k' t' t_wr' rts')" oops
+
+lemma read_prepare_write_indep:
+  "cl \<noteq> get_cl_w t' \<Longrightarrow> t \<noteq> t' \<Longrightarrow> left_commute tps (Read cl k v t) (PrepW k' t' v')" oops
+
+lemma read_commit_write_indep:
+  "cl \<noteq> get_cl_w t \<Longrightarrow> left_commute tps (Read cl k v t) (CommitW k' t' v' cts')" oops
+
+
+\<comment> \<open>read_done\<close>
+
+lemma read_done_read_done_indep:
+  "cl \<noteq> cl' \<Longrightarrow> left_commute tps (RDone cl kv_map sn u'') (RDone cl' kv_map' sn' u''')"
+  apply (auto simp add: left_commute_def tps_trans_defs get_ctx_defs del: equalityI)
+  apply (rule relcompI, auto)
+  by (simp add: fun_upd_twist)
+
+lemma read_done_write_invoke_indep:
+  "cl \<noteq> cl' \<Longrightarrow> left_commute tps (RDone cl kv_map sn u'') (WInvoke cl' kv_map')"
+  apply (auto simp add: left_commute_def tps_trans_defs get_ctx_defs del: equalityI)
+  apply (rule relcompI, auto)
+  by (simp add: fun_upd_twist)
+
+lemma read_done_write_commit_indep:
+  "cl \<noteq> cl' \<Longrightarrow> left_commute tps (RDone cl kv_map sn u'') (WCommit cl' kv_map' cts' sn' u''')"
+  apply (auto simp add: left_commute_def tps_trans_defs get_ctx_defs ext_corder_def del: equalityI)
+  apply (rule relcompI, auto) oops
+
+lemma read_done_write_done_indep:
+  assumes "cl \<noteq> cl'"
+  shows "left_commute tps (RDone cl kv_map sn u'') (WDone cl' kv_map')"
+  apply (auto simp add: left_commute_def tps_trans_defs get_ctx_defs del: equalityI)
+  apply (rule relcompI, auto) oops
+
+lemma read_done_register_read_indep:
+  "cl \<noteq> get_cl t' \<Longrightarrow> left_commute tps (RDone cl kv_map sn u'') (RegR k' t' t_wr' rts')" oops
+
+lemma read_done_prepare_write_indep:
+  "cl \<noteq> get_cl_w t' \<Longrightarrow> left_commute tps (RDone cl kv_map sn u'') (PrepW k' t' v')" oops
+
+lemma read_done_commit_write_indep:
+  "cl \<noteq> get_cl_w t \<Longrightarrow> left_commute tps (RDone cl kv_map sn u'') (CommitW k' t' v' cts')" oops
+
+
+\<comment> \<open>write_invoke\<close>
+
+lemma write_invoke_write_invoke_indep:
+  "cl \<noteq> cl' \<Longrightarrow> left_commute tps (WInvoke cl kv_map) (WInvoke cl' kv_map')"
+  apply (auto simp add: left_commute_def tps_trans_defs del: equalityI)
+  apply (rule relcompI, auto)
+  by (simp add: fun_upd_twist)
+
+lemma write_invoke_write_commit_indep:
+  "cl \<noteq> cl' \<Longrightarrow> left_commute tps (WInvoke cl kv_map) (WCommit cl' kv_map' cts' sn' u''')"
+  apply (auto simp add: left_commute_def tps_trans_defs del: equalityI)
+  apply (rule relcompI, auto)
+  apply (simp add: fun_upd_twist)
+  by (metis domI option.inject)
+
+lemma write_invoke_write_done_indep:
+  assumes "cl \<noteq> cl'"
+  shows "left_commute tps (WInvoke cl kv_map) (WDone cl' kv_map')"
+  apply (auto simp add: left_commute_def tps_trans_defs del: equalityI)
+  apply (rule relcompI, auto)
+  using assms apply fastforce oops
+
+lemma write_invoke_register_read_indep:
+  "cl \<noteq> get_cl t' \<Longrightarrow> left_commute tps (WInvoke cl kv_map) (RegR k' t' t_wr' rts')" oops
+
+lemma write_invoke_prepare_write_indep:
+  "cl \<noteq> get_cl_w t' \<Longrightarrow> left_commute tps (WInvoke cl kv_map) (PrepW k' t' v')" oops
+
+lemma write_invoke_commit_write_indep:
+  "cl \<noteq> get_cl_w t \<Longrightarrow> left_commute tps (WInvoke cl kv_map) (CommitW k' t' v' cts')" oops
+
+
+\<comment> \<open>write_commit\<close>
+
+lemma write_commit_write_commit_indep:
+  "cl \<noteq> cl' \<Longrightarrow> left_commute tps (WCommit cl kv_map cts sn u'') (WCommit cl' kv_map' cts' sn' u''')"
+  apply (auto simp add: left_commute_def tps_trans_defs del: equalityI)
+  apply (rule relcompI, auto) oops
+
+lemma write_commit_write_done_indep:
+  assumes "cl \<noteq> cl'"
+  shows "left_commute tps (WCommit cl kv_map cts sn u'') (WDone cl' kv_map')"
+  apply (auto simp add: left_commute_def tps_trans_defs get_ctx_defs del: equalityI)
+  apply (rule relcompI, auto) oops
+
+lemma write_commit_register_read_indep:
+  "cl \<noteq> get_cl t' \<Longrightarrow> left_commute tps (WCommit cl kv_map cts sn u'') (RegR k' t' t_wr' rts')" oops
+
+lemma write_commit_prepare_write_indep:
+  "cl \<noteq> get_cl_w t' \<Longrightarrow> left_commute tps (WCommit cl kv_map cts sn u'') (PrepW k' t' v')" oops
+
+lemma write_commit_commit_write_indep:
+  "cl \<noteq> get_cl_w t' \<Longrightarrow> left_commute tps (WCommit cl kv_map cts sn u'') (CommitW k' t' v' cts')" oops
+
+
+end
